theories/examples/susp_correctness/definitions.v
@@ -1,0 +1,378 @@
+From auth.prelude Require Import stdpp.
+From auth.heap_lang Require Import typedproph.
+From auth.heap_lang.lib Require Import serialization_susp list.
+From auth.examples.susp_correctness Require Import resource_algebras.
+
+(** * Prophesied stream *)
+Section proph.
+  Context `{heapGS Σ}.
+
+  Fixpoint take_until {A B : Type} (f : A → option B) (xs : list A) : list B :=
+    match xs with
+    | []      => []
+    | x :: xs =>
+      match f x with
+      | Some y => y :: (take_until f xs)
+      | None   => []
+      end
+    end.
+
+  Definition longest_valid_prefix_bool (us : list val) : list bool :=
+    take_until (λ u, match u with InjRV (LitV (LitBool b)) => Some b | _ => None end) us.
+
+  Definition proph_bs (p : proph_id) (bs : list bool) : iProp Σ :=
+    (∃ (us : list (val * val)), proph p us ∗ ⌜bs = longest_valid_prefix_bool (map snd us)⌝)%I.
+
+  Definition longest_valid_prefix_string (us : list val) : list string :=
+    take_until (λ u, match u with InjRV (LitV (LitString s)) => Some s | _ => None end) us.
+
+  Definition proph_proof (p : proph_id) (vs : list string) : iProp Σ :=
+    (∃ (us : list (val * val)), proph p us ∗ ⌜vs = longest_valid_prefix_string (map snd us)⌝)%I.
+
+  Definition longest_valid_prefix_val (us : list val) : list val :=
+    take_until (λ u, match u with InjRV v => Some v | _ => None end) us.
+
+  Definition proph_as (p : proph_id) (vs : list val) : iProp Σ :=
+    (∃ (us : list (val * val)), proph p us ∗ ⌜vs = longest_valid_prefix_val (map snd us)⌝)%I.
+
+  Lemma wp_resolve_proph_bool p bs (b : bool) :
+    {{{ proph_bs p bs }}}
+      resolve_proph: #p to: (SOMEV #b)
+    {{{ bs', RET #(); ⌜bs = b :: bs'⌝ ∗ proph_bs p bs' }}}.
+  Proof.
+    iIntros (Φ) "(%us & Hp & %) HΦ".
+    wp_apply (wp_resolve_proph with "Hp").
+    iIntros (?) "[% Hp]". iApply "HΦ".
+    iFrame. by simplify_eq.
+  Qed.
+
+  Lemma wp_resolve_proph_nil_bool p bs :
+    {{{ proph_bs p bs }}} resolve_proph: #p to: NONEV {{{ RET #(); ⌜bs = []⌝ }}}.
+  Proof.
+    iIntros (Φ) "(%us & Hp & %) HΦ".
+    wp_apply (wp_resolve_proph with "Hp").
+    iIntros (?) "[% Hp]". iApply "HΦ".
+    by simplify_eq.
+  Qed.
+
+  Lemma wp_resolve_proph_string p vs (s : string) :
+    {{{ proph_proof p vs }}}
+      resolve_proph: #p to: (SOMEV #s)
+    {{{ vs', RET #(); ⌜vs = s :: vs'⌝ ∗ proph_proof p vs' }}}.
+  Proof.
+    iIntros (Φ) "(%us & Hp & %) HΦ".
+    wp_apply (wp_resolve_proph with "Hp").
+    iIntros (?) "[% Hp]". iApply "HΦ".
+    iFrame. by simplify_eq.
+  Qed.
+
+  Lemma wp_resolve_proph_nil_string p vs :
+    {{{ proph_proof p vs }}} resolve_proph: #p to: NONEV {{{ RET #(); ⌜vs = []⌝ }}}.
+  Proof.
+    iIntros (Φ) "(%us & Hp & %) HΦ".
+    wp_apply (wp_resolve_proph with "Hp").
+    iIntros (?) "[% Hp]". iApply "HΦ".
+    by simplify_eq.
+  Qed.
+
+  Lemma wp_resolve_proph_val p vs (v : val) :
+    {{{ proph_as p vs }}}
+      resolve_proph: #p to: (SOMEV v)
+    {{{ vs', RET #(); ⌜vs = v :: vs'⌝ ∗ proph_as p vs' }}}.
+  Proof.
+    iIntros (Φ) "(%us & Hp & %) HΦ".
+    wp_apply (wp_resolve_proph with "Hp").
+    iIntros (?) "[% Hp]". iApply "HΦ".
+    iFrame. by simplify_eq.
+  Qed.
+
+  Lemma wp_resolve_proph_nil_val p vs :
+    {{{ proph_as p vs }}} resolve_proph: #p to: NONEV {{{ RET #(); ⌜vs = []⌝ }}}.
+  Proof.
+    iIntros (Φ) "(%us & Hp & %) HΦ".
+    wp_apply (wp_resolve_proph with "Hp").
+    iIntros (?) "[% Hp]". iApply "HΦ".
+    by simplify_eq.
+  Qed.
+
+  Definition is_proof (v : val) (ps : list string) : Prop :=
+    is_list ps v.
+
+  Definition is_proph_proof (v : val) (p : proph_id) (ps : list string) : iProp Σ :=
+    ⌜is_proof v ps⌝ ∗ proph_proof p ps.
+
+End proph.
+
+
+Definition prover_susp_set (N : namespace) : namespace := N .@ "psusp".
+Definition prover_susp_n (N : namespace) (v : val) : namespace := (prover_susp_set N) .@ v.
+
+Definition ver_susp_set (N : namespace) : namespace := N .@ "vsusp".
+Definition ver_susp_n (N : namespace) (v : val) : namespace := (ver_susp_set N) .@ v.
+
+Section authenticatable_definitions.
+  Context `{!authG Σ, !seqG Σ, !visited_mapG Σ, !lg_mapG Σ, !mapG Σ, !capG Σ} (N : namespace).
+
+  Inductive evi_type : Type :=
+  | tprod (t1 t2 : evi_type)
+  | tsum (t1 t2 : evi_type)
+  | tstring
+  | tint
+  | tauth.
+
+  #[global] Instance : Inhabited evi_type.
+  Proof. constructor. apply tstring. Qed.
+
+  (* For verifier *)
+  Fixpoint sub_obj (t : evi_type) (v sv: val) :=
+    match t with
+    | tprod t1 t2 =>
+        ∃ v1 v2, v = (v1, v2)%V ∧ (sv = v1 ∨ sv = v2 ∨ sub_obj t1 v1 sv ∨ sub_obj t2 v2 sv)
+    | tsum t1 t2 =>
+        ∃ v', ((v = InjLV v' ∧ sub_obj t1 v' sv ∧ v = v') ∨
+                 (v = InjRV v' ∧ sub_obj t2 v' sv ∧ v = v'))
+    | tstring => False
+    | tint => False
+    | tauth =>
+        ∃ v', (v = SOMEV (InjLV v') ∨ (v = SOMEV (InjRV v'))) ∧ v' = sv
+  end.
+
+  Definition suspended_string : string := none_ser_str.
+
+  Definition simple_string (s : string) : string := string_ser_str s.
+
+  Definition filled_string (s : string) : string := some_ser_str (simple_string s).
+
+  Definition empty_proph_bs (p : proph_id) : iProp Σ :=
+    proph_bs p [].
+
+  Definition fill_proph_bs (p : proph_id) (bs : list bool) : iProp Σ :=
+    proph_bs p bs ∗ ⌜~ In true bs⌝.
+
+  Definition unfill_proph_bs (p : proph_id) (bs : list bool) : iProp Σ :=
+    proph_bs p bs ∗ ⌜∃ bs', bs = true :: bs'⌝.
+
+  (* Definition proph_p_susp (p : proph_id) (bs : bool list) : iProp Σ :=
+    (typed_proph_prop IntTypedProph) p bs. *)
+
+  Definition proph_v_susp (p : proph_id) (s : string) : iProp Σ :=
+    (typed_proph1_prop StringTypedProph) p s.
+
+  (* Definition auth_p_unsusp (v : val) : iProp Σ :=
+    ∃ (a : val) (s : string), 
+      ⌜v = (a, #(hash s))%V⌝ ∗ hashed s ∗
+      s_is_ser (g:=gwp_upto_bad) auth_scheme a s.
+
+  (* ps true denotes going to suspend, false otherwise *)
+  Definition auth_p_susp (v : val) : iProp Σ :=
+    ∃ (b r ord : bool) (lb lr : loc) (ps : proph_id) (a : val) (s : string),
+      ⌜v = (#ps, #lb, #lr, a, #(hash s))%V⌝ ∗ hashed s ∗
+      lb ↦ #b ∗ lb ↦ #r ∗ proph_susp ps ord ∗
+      s_is_ser (g:=gwp_upto_bad) auth_scheme a s. *)
+
+  Definition auth_unsusp_ser_p (v : val) (s : string) : iProp Σ :=
+    ∃ (a : val) (h : string),
+      ⌜v = (a, #h)%V ∧ s = simple_string h⌝.
+
+  Definition susp_p_fill_inv (ps : proph_id) (lb lr : loc) : iProp Σ :=
+    lb ↦ #false ∗ ((∃ (bs : list bool), lr ↦ #false ∗ fill_proph_bs ps bs) ∨
+      (lr ↦ #true ∗ empty_proph_bs ps)).
+
+  Definition auth_susp_ser_p_fill (v : val) (s : string) : iProp Σ :=
+    ∃ (p : proph_id) (lb lr : loc) (a : val) (h : string) (r : bool),
+      ⌜v = (#lb, #lr, a, #h, #p)%V ∧ s = simple_string h⌝ ∗
+      seq_inv (prover_susp_n N v) (susp_p_fill_inv p lb lr).
+
+  Definition susp_p_unfill_inv (ps : proph_id) (lb lr : loc) : iProp Σ :=
+    ∃ (γ : gname), (* 1-1 relation between lb, γ and pid *)
+      lg_mapg_frag lb γ ∗
+      ((∃ (bs : list bool),
+        lb ↦ #false ∗ lr ↦ #false ∗ unfill_proph_bs ps bs ∗ visit_pending γ) ∨
+      (∃ (r : bool) (bs : list bool) (n : nat),
+        lb ↦ #true ∗ lr ↦ #r ∗ proph_bs ps bs ∗ visit_reached_done γ n)).
+
+  Definition auth_susp_ser_p_emp (v : val) (s : string) : iProp Σ :=
+    ∃ (p : proph_id) (lb lr : loc) (a : val) (h : string) (r : bool),
+      ⌜v = (#lb, #lr, a, #h, #p)%V ∧ s = suspended_string⌝ ∗
+      seq_inv (prover_susp_n N v) (susp_p_unfill_inv p lb lr).
+
+  (* What it will actually serialize to *)
+  Definition auth_susp_ser_p_real (v : val) (s : string) : iProp Σ :=
+    auth_susp_ser_p_fill v s ∨ auth_susp_ser_p_emp v s.
+
+  (* What it would serialize to without suspension *)
+  Definition auth_susp_ser_p (v : val) (s : string) : iProp Σ :=
+    ∃ (p : proph_id) (lb lr : loc) (a : val) (h : string),
+      ⌜v = (#lb, #lr, a, #h, #p)%V ∧ s = simple_string h⌝.
+
+  Definition auth_fill_ser_v (v : val) (s : string) : iProp Σ :=
+    ∃ (h : string), ⌜s = filled_string h ∧ v = InjLV #h⌝.
+
+  Definition auth_susp_fill_v (v : val) (s : string) : iProp Σ :=
+    ∃ (h : string) (susp : loc) γ n, 
+      ⌜s = filled_string h ∧ v = InjRV #susp⌝ ∗ susp ↦ᵥ{#(3/4)} InjRV #h ∗
+      lg_mapg_frag susp γ ∗ visit_finished γ n.
+
+  (* Definition auth_susp_emp_v (v : val) (s : string) : iProp Σ :=
+    ∃ (h : string) (susp : loc) (pid: nat) (p : proph_id),
+      ⌜s = suspended_string ∧ v = InjRV #susp⌝ ∗ 
+      susp ↦ᵥ{#(3/4)} InjLV (#pid, #p) ∗ proph_v_susp p h. *)
+
+  Definition auth_susp_emp_v_proph (v : val) : iProp Σ :=
+    ∃ (h : string) (susp : loc) (pid: nat) (p : proph_id) pv pt (q : Qp) γ,
+      ⌜v = InjRV #susp⌝ ∗ mapg_frag #pid q pv ∗ lg_mapg_frag susp γ ∗
+      ⌜sub_obj pt pv v⌝ ∗ susp ↦ᵥ{#(3/4)} InjLV (#pid, #p) ∗ proph_v_susp p h.
+
+  Definition auth_susp_v_ser_proph_inv (v : val) (s : string) : iProp Σ :=
+    (∃ (s1 : string), 
+      ⌜s = filled_string (hash s1)⌝ ∗
+      auth_susp_fill_v v s) ∨ 
+    auth_susp_emp_v_proph v.
+
+  Definition auth_susp_v_ser_proph (v : val) (s : string) : iProp Σ :=
+    seq_inv (ver_susp_n N v) (auth_susp_v_ser_proph_inv v s).
+
+  Fixpoint unsusp (t : evi_type) (v un_v : val) : Prop :=
+    match t with
+    | tprod t1 t2 =>
+      ∃ v1 v2 un_v1 un_v2,
+        v = (v1, v2)%V ∧ un_v = (un_v1, un_v2)%V ∧
+          unsusp t1 v1 un_v1 ∧ unsusp t2 v2 un_v2
+    | tsum t1 t2 =>
+      (∃ v1 un_v1,
+        v = InjLV v1 ∧ un_v = InjLV un_v1 ∧ unsusp t1 v1 un_v1) ∨
+      (∃ v2 un_v2,
+        v = InjRV v2 ∧ un_v = InjRV un_v2 ∧ unsusp t2 v2 un_v2)
+    | tstring | tint => v = un_v
+    | tauth =>
+      ∃ (lb lr : loc) (a : val) (h : string) (p : proph_id),
+        v = (#lb, #lr, a, #h, #p)%V ∧ un_v = (a, #h)%V
+    end.
+
+  (* unsuspended *)
+  Fixpoint unsusp_ser_p (t : evi_type) (v : val) (s : string) : iProp Σ :=
+    match t with
+    | tprod t1 t2 => prod_is_ser' v s (unsusp_ser_p t1) (unsusp_ser_p t2)
+    | tsum t1 t2 => sum_is_ser' v s (unsusp_ser_p t1) (unsusp_ser_p t2)
+    | tstring => string_is_ser v s
+    | tint => int_is_ser v s
+    | tauth => auth_unsusp_ser_p v s
+    end.
+
+  #[global] Instance unsusp_ser_p_persistent t v s : Persistent (unsusp_ser_p t v s).
+  Proof. revert v s. induction t => v s; simpl; apply _. Qed.
+
+  (* suspended real *)
+  Fixpoint susp_ser_p_real (t : evi_type) (v : val) (s : string) : iProp Σ :=
+    match t with
+    | tprod t1 t2 => prod_is_ser' v s (susp_ser_p_real t1) (susp_ser_p_real t2)
+    | tsum t1 t2 => sum_is_ser' v s (susp_ser_p_real t1) (susp_ser_p_real t2)
+    | tstring => string_is_ser v s
+    | tint => int_is_ser v s
+    | tauth => auth_susp_ser_p_real v s
+    end.
+ 
+  #[global] Instance susp_ser_p_real_persistent t v s : Persistent (susp_ser_p_real t v s).
+  Proof. revert v s. induction t => v s; simpl; apply _. Qed.
+
+  (* suspended proph *)
+  Fixpoint susp_ser_p (t : evi_type) (v : val) (s : string) : iProp Σ :=
+    match t with
+    | tprod t1 t2 => prod_is_ser' v s (susp_ser_p t1) (susp_ser_p t2)
+    | tsum t1 t2 => sum_is_ser' v s (susp_ser_p t1) (susp_ser_p t2)
+    | tstring => string_is_ser v s
+    | tint => int_is_ser v s
+    | tauth => auth_susp_ser_p v s
+    end.
+ 
+  #[global] Instance susp_ser_p_proph_persistent t v s : Persistent (susp_ser_p t v s).
+  Proof. revert v s. induction t => v s; simpl; apply _. Qed.
+
+  Fixpoint ser_v (t : evi_type) (v : val) (s : string) : iProp Σ :=
+    match t with
+    | tprod t1 t2 => prod_is_ser' v s (ser_v t1) (ser_v t2)
+    | tsum t1 t2 => sum_is_ser' v s (ser_v t1) (ser_v t2)
+    | tstring => string_is_ser v s
+    | tint => int_is_ser v s
+    | tauth => ∃ v1, ⌜v = SOMEV v1⌝ ∗ auth_fill_ser_v v1 s
+    end.
+ 
+  #[global] Instance ser_v_persistent t v s : Persistent (ser_v t v s).
+  Proof. revert v s. induction t => v s; simpl; apply _. Qed.
+
+  Fixpoint ser_v_proph (t : evi_type) (v : val) (s : string) : iProp Σ :=
+    match t with
+    | tprod t1 t2 => prod_is_ser' v s (ser_v_proph t1) (ser_v_proph t2)
+    | tsum t1 t2 => sum_is_ser' v s (ser_v_proph t1) (ser_v_proph t2)
+    | tstring => string_is_ser v s
+    | tint => int_is_ser v s
+    | tauth => ∃ v1, ⌜v = SOMEV v1⌝ ∗
+                       (auth_fill_ser_v v1 s ∨ auth_susp_v_ser_proph v1 s)
+  end.
+ 
+  #[global] Instance ser_v_proph_persistent t v s : Persistent (ser_v_proph t v s).
+  Proof. revert v s. induction t => v s; simpl; apply _. Qed.
+
+  (* For both prover/verifier
+  Fixpoint invalid_value (t : evi_type) (v : val) :=
+    match t with
+    | tprod t1 t2 =>
+      ∃ v1 v2, v = (v1, v2)%V ∧ (invalid_value t1 v1 ∨ invalid_value t2 v2)
+    | tsum t1 t2 =>
+      (∃ v1, v = InjLV v1 ∧ invalid_value t1 v1) ∨
+      (∃ v2, v = InjLV v2 ∧ invalid_value t2 v2)
+    | tstring => False
+    | tint => False
+    | tauth => v = NONEV
+    end. *)
+
+  (* Tauth leaf with fragment: unfilled susps carry a [1/N] piece of
+     [mapg_frag #pid _ v_outer]. [N] is the total number of B2 leaves
+     created at deser time; [v_outer] is the outer value. *)
+  Definition auth_sub_susp_count_frags
+      (v : val) (c pid N : nat) (v_outer : val) : iProp Σ :=
+    ∃ v1, ⌜v = SOMEV v1⌝ ∧
+      ((∃ (h : string), ⌜v1 = InjLV #h ∧ c = 0⌝) ∨
+        (∃ (susp : loc),
+          ⌜v1 = InjRV #susp⌝ ∗
+            ((∃ (h : string), susp ↦ᵥ{#1/4} (InjRV #h) ∗ ⌜c = 0⌝) ∨
+              (∃ (p : proph_id) γ,
+                lg_mapg_frag susp γ ∗
+                susp ↦ᵥ{#1/4} InjLV (#pid, #p) ∗ ⌜c = 1⌝ ∗
+                mapg_frag #pid (1 / pos_to_Qp (Pos.of_nat N))%Qp v_outer ∗
+                cap_frag pid N ∗
+                (visit_pending γ ∨ ∃ id, ⌜id > pid⌝ ∗ visit_done γ id))))).
+
+  Fixpoint sub_susp_count
+      (t : evi_type) (v : val) (c id N : nat) (v_outer : val) : iProp Σ :=
+    match t with
+    | tprod t1 t2 =>
+        ∃ (c1 c2 : nat) (v1 v2 : val),
+          ⌜v = (v1, v2)%V ∧ (c1 + c2)%nat = c⌝ ∗
+          sub_susp_count t1 v1 c1 id N v_outer ∗
+          sub_susp_count t2 v2 c2 id N v_outer
+    | tsum t1 t2 =>
+        (∃ (v1 : val), ⌜v = InjLV v1⌝ ∗ sub_susp_count t1 v1 c id N v_outer) ∨
+        (∃ (v2 : val), ⌜v = InjRV v2⌝ ∗ sub_susp_count t2 v2 c id N v_outer)
+    | tstring => string_valid_val v ∧ ⌜c = 0⌝
+    | tint => int_valid_val v ∧ ⌜c = 0⌝
+    | tauth => auth_sub_susp_count_frags v c id N v_outer
+    end.
+
+  (* Accumulated fragment at the top level. The invariant is that every
+     filled susp has returned its [1/N] piece here, so the aggregator holds
+     [(N - c)/N]. When [c = N] nothing has been returned yet (left disjunct,
+     no fragment). When [c = 0] the aggregator holds the full fraction. *)
+  Definition count_aggregator (c id N : nat) (v : val) : iProp Σ :=
+    ⌜c = N⌝ ∨
+    (⌜c < N⌝ ∗ ∃ q,
+      ⌜(q * pos_to_Qp (Pos.of_nat N))%Qp = pos_to_Qp (Pos.of_nat (N - c))⌝ ∗
+      mapg_frag #id q v).
+
+  Definition sub_susp_count_frags
+      (t : evi_type) (v : val) (c id N : nat) : iProp Σ :=
+    cap_frag id N ∗ ⌜c ≤ N⌝ ∗
+    sub_susp_count t v c id N v ∗
+    count_aggregator c id N v.
+End authenticatable_definitions.
+  
