theories/examples/susp_correctness/resource_algebras.v
@@ -1,0 +1,460 @@
+From auth.prelude Require Import stdpp.
+From auth.rel_logic_tern_susp Require Export model.
+From iris.algebra Require Import gmap auth.
+From iris.algebra.lib Require Import dfrac_agree.
+
+(* Nat is going to be the id assigned by the verifier. We are going to show that
+  for some value in the verifier's map, the ctr must be > 0. These values are either
+  yet to be seen or are in the map. visit_done denotes values have been seen.
+  In the end we will say that for the highest id value in the map all values must
+  have been seen (because of flush_buf_stream), and since this is the highest
+  id, and children's ids are higher, we have a contradiction. *)
+Definition visited_state_mapUR :=
+  authUR (gmap gname (dfrac_agreeR (optionUR (prodUR natO (optionUR unitO))))).
+Definition visited_done_mapUR :=
+  authUR (gmap gname (agreeR natO)).
+Class visited_mapG Σ := VisitedMapG {
+  visited_state_inG :> inG Σ visited_state_mapUR;
+  visited_done_inG :> inG Σ visited_done_mapUR;
+  visited_state_name : gname;
+  visited_done_name : gname;
+}.
+
+Section visited_map_res.
+  Context `{!visited_mapG Σ}.
+
+  Definition state_val_type := dfrac_agreeR (option (nat * option unit)).
+  Definition state_mapg_type := gmap gname state_val_type.
+  Definition done_mapg_type := gmap gname (agreeR natO).
+
+  Definition pending_val : state_val_type :=
+    to_dfrac_agree (DfracOwn (1/2)%Qp) None.
+
+  Definition pending_val_full : state_val_type :=
+    to_dfrac_agree (DfracOwn 1) None.
+
+  Definition done_val n : state_val_type :=
+    to_dfrac_agree (DfracOwn 1) (Some (n, None)).
+
+  Definition finished_val n : state_val_type :=
+    to_dfrac_agree DfracDiscarded (Some (n, Some ())).
+
+  Definition visited_coherent (m : state_mapg_type) (d : done_mapg_type) : Prop :=
+    ∀ γ, d !! γ ≠ None →
+      ∃ n, m !! γ = Some (done_val n) ∨ m !! γ = Some (finished_val n).
+
+  Definition visited_mapg_auth (m : state_mapg_type) (d : done_mapg_type) : iProp Σ :=
+    own visited_state_name (● m) ∗ own visited_done_name (● d) ∗
+    ⌜visited_coherent m d⌝.
+
+  Definition visited_map_update_pending
+      (m : state_mapg_type) (d : done_mapg_type) γ : iProp Σ :=
+    own visited_state_name (● <[ γ := pending_val_full ]>m) ∗
+    own visited_done_name (● d) ∗
+    ⌜visited_coherent (<[ γ := pending_val_full ]>m) d⌝.
+
+  Definition visited_map_update_done
+      (m : state_mapg_type) (d : done_mapg_type) γ n : iProp Σ :=
+    own visited_state_name (● <[ γ := done_val n ]>m) ∗
+    own visited_done_name (● <[ γ := to_agree n ]>d) ∗
+    ⌜visited_coherent (<[ γ := done_val n ]>m) (<[ γ := to_agree n ]>d)⌝.
+
+  Definition visited_map_update_finished
+      (m : state_mapg_type) (d : done_mapg_type) γ n : iProp Σ :=
+    own visited_state_name (● <[ γ := finished_val n ]>m) ∗
+    own visited_done_name (● d) ∗
+    ⌜visited_coherent (<[ γ := finished_val n ]>m) d⌝.
+
+  Definition visit_pending γ : iProp Σ :=
+    own visited_state_name (◯ {[ γ := pending_val ]}).
+
+  Definition visit_reached_done γ n : iProp Σ :=
+    own visited_done_name (◯ {[ γ := to_agree n ]}).
+
+  Definition visit_done γ n : iProp Σ :=
+    own visited_state_name (◯ {[ γ := done_val n ]}) ∗ visit_reached_done γ n.
+
+  Definition visit_finished γ n : iProp Σ :=
+    own visited_state_name (◯ {[ γ := finished_val n ]}) ∗ visit_reached_done γ n.
+
+  Global Instance visit_reached_done_persistent γ n :
+    Persistent (visit_reached_done γ n).
+  Proof. rewrite /visit_reached_done. apply _. Qed.
+
+  Global Instance visit_finished_persistent γ n :
+    Persistent (visit_finished γ n).
+  Proof. rewrite /visit_finished /finished_val. apply _. Qed.
+
+  Local Lemma pending_val_split :
+    pending_val ⋅ pending_val ≡ pending_val_full.
+  Proof.
+    rewrite /pending_val /pending_val_full -dfrac_agree_op dfrac_op_own Qp.half_half //.
+  Qed.
+
+  Lemma visited_insert m d γ :
+    m !! γ = None →
+    visited_mapg_auth m d ==∗
+      visited_map_update_pending m d γ ∗ visit_pending γ ∗ visit_pending γ.
+  Proof.
+    iIntros (Hfresh) "(Hms & Hd & %Hcoh)".
+    rewrite /visited_map_update_pending /visit_pending.
+    iMod (own_update _ _
+      (● <[γ := pending_val_full]>m
+        ⋅ (◯ {[γ := pending_val]} ⋅ ◯ {[γ := pending_val]}))
+      with "Hms") as "[$ [$ $]]".
+    { rewrite -auth_frag_op singleton_op pending_val_split.
+      apply auth_update_alloc, alloc_singleton_local_update; [done|].
+      rewrite /pending_val_full pair_valid; done. }
+    iFrame "Hd". iPureIntro.
+    intros γ' Hdγ'. destruct (decide (γ' = γ)) as [-> | Hne].
+    - destruct (Hcoh γ Hdγ') as (n & [Heq | Heq]); rewrite Hfresh in Heq; discriminate.
+    - rewrite lookup_insert_ne; [|done]. by apply Hcoh.
+  Qed.
+
+  Lemma visited_transition_done m d γ n :
+    d !! γ = None →
+    visited_mapg_auth m d -∗ visit_pending γ -∗ visit_pending γ
+    ==∗ visited_map_update_done m d γ n ∗ visit_done γ n.
+  Proof.
+    iIntros (Hfresh) "(Hms & Hd & %Hcoh) H1 H2".
+    rewrite /visited_map_update_done /visit_pending /visit_done /visit_reached_done.
+    iMod (own_update_3 _ _ _ _
+      (● <[γ := done_val n]>m ⋅ ◯ {[γ := done_val n]})
+      with "Hms H1 H2") as "[$ Hsfrag]".
+    { rewrite -assoc -auth_frag_op singleton_op pending_val_split.
+      apply auth_update, singleton_local_update_any.
+      intros x Hx. apply exclusive_local_update.
+      rewrite /done_val pair_valid; done. }
+    iMod (own_update _ _
+      (● <[γ := to_agree n]>d ⋅ ◯ {[γ := to_agree n]})
+      with "Hd") as "[$ #$]".
+    { apply auth_update_alloc, alloc_singleton_local_update; done. }
+    iFrame "Hsfrag". iPureIntro.
+    intros γ' Hdγ'. destruct (decide (γ' = γ)) as [-> | Hne].
+    - exists n. left. by rewrite lookup_insert.
+    - rewrite lookup_insert_ne in Hdγ'; [|done].
+      rewrite lookup_insert_ne; [|done]. by apply Hcoh.
+  Qed.
+
+  Lemma visited_transition_finished m d γ n :
+    visited_mapg_auth m d -∗ visit_done γ n
+    ==∗ visited_map_update_finished m d γ n ∗ visit_finished γ n.
+  Proof.
+    iIntros "(Hms & Hd & %Hcoh) [Hsfrag #Hreached]".
+    rewrite /visited_map_update_finished /visit_finished /visit_reached_done.
+    iAssert (⌜d !! γ ≠ None⌝)%I as %Hdγ.
+    { iDestruct (own_valid_2 with "Hd Hreached") as %Hv.
+      apply auth_both_valid_discrete in Hv as [Hincl _].
+      apply singleton_included_l in Hincl as (xd & Hxd & _).
+      iPureIntro. intros Heq. rewrite Heq in Hxd. inversion Hxd. }
+    iMod (own_update_2 _ _ _
+      (● <[γ := finished_val n]>m ⋅ ◯ {[γ := finished_val n]})
+      with "Hms Hsfrag") as "[$ $]".
+    { apply auth_update, singleton_local_update_any.
+      intros x Hx. apply exclusive_local_update.
+      rewrite /finished_val pair_valid; done. }
+    iFrame "Hd Hreached". iPureIntro.
+    intros γ' Hdγ'. destruct (decide (γ' = γ)) as [-> | Hne].
+    - exists n. right. by rewrite lookup_insert.
+    - rewrite lookup_insert_ne; [|done]. by apply Hcoh.
+  Qed.
+
+  Lemma visit_done_keep γ n :
+    visit_done γ n ⊢ visit_done γ n ∗ visit_reached_done γ n.
+  Proof.
+    iIntros "[Hs #Hr]". iFrame "Hs Hr Hr".
+  Qed.
+
+  Lemma visit_finished_keep γ n :
+    visit_finished γ n ⊢ visit_finished γ n ∗ visit_reached_done γ n.
+  Proof.
+    iIntros "[Hs #Hr]". iFrame "Hs Hr Hr".
+  Qed.
+
+  Lemma visited_invalid_1 γ n :
+    visit_pending γ ∗ visit_done γ n -∗ False.
+  Proof.
+    rewrite /visit_pending /visit_done.
+    iIntros "[H1 [H2 _]]". iCombine "H1 H2" as "H".
+    iDestruct (own_valid with "H") as %Hv. iPureIntro.
+    rewrite auth_frag_valid singleton_valid in Hv.
+    rewrite /pending_val /done_val in Hv.
+    by apply dfrac_agree_op_valid_L in Hv as [_ ?].
+  Qed.
+
+  Lemma visited_invalid_2 γ n :
+    visit_pending γ ∗ visit_finished γ n -∗ False.
+  Proof.
+    rewrite /visit_pending /visit_finished.
+    iIntros "[H1 [H2 _]]". iCombine "H1 H2" as "H".
+    iDestruct (own_valid with "H") as %Hv. iPureIntro.
+    rewrite auth_frag_valid singleton_valid in Hv.
+    rewrite /pending_val /finished_val in Hv.
+    by apply dfrac_agree_op_valid_L in Hv as [_ ?].
+  Qed.
+
+  Lemma visited_invalid_3 γ n1 n2 :
+    visit_done γ n1 ∗ visit_finished γ n2 -∗ False.
+  Proof.
+    rewrite /visit_done /visit_finished.
+    iIntros "[[H1 _] [H2 _]]". iCombine "H1 H2" as "H".
+    iDestruct (own_valid with "H") as %Hv. iPureIntro.
+    rewrite auth_frag_valid singleton_valid in Hv.
+    rewrite /done_val /finished_val in Hv.
+    apply dfrac_agree_op_valid_L in Hv as [_ Heq]. by simplify_eq.
+  Qed.
+
+  Lemma visited_reached_done_agree γ n1 n2 :
+    visit_reached_done γ n1 -∗ visit_reached_done γ n2 -∗ ⌜n1 = n2⌝.
+  Proof.
+    rewrite /visit_reached_done.
+    iIntros "H1 H2".
+    iDestruct (own_valid_2 with "H1 H2") as %Hv. iPureIntro.
+    rewrite -auth_frag_op singleton_op auth_frag_valid singleton_valid in Hv.
+    by apply to_agree_op_inv_L in Hv.
+  Qed.
+
+  Lemma get_visit_reached_done γ n m d :
+    d !! γ = Some (to_agree n) →
+    visited_mapg_auth m d ==∗ visited_mapg_auth m d ∗ visit_reached_done γ n.
+  Proof.
+    iIntros (Hd) "(Hms & Hd & %Hcoh)".
+    rewrite /visit_reached_done.
+    iMod (own_update _ _ (● d ⋅ ◯ {[γ := to_agree n]}) with "Hd") as "[Hd #Hr]".
+    { apply auth_update_dfrac_alloc; [apply _|].
+      apply singleton_included_l. exists (to_agree n). split; [by rewrite Hd|].
+      apply Some_included_2. by left. }
+    iModIntro. by iFrame "∗ # %".
+  Qed.
+
+  Lemma visited_reached_done_invalid γ n m d :
+    visited_mapg_auth m d -∗ visit_reached_done γ n -∗ visit_pending γ -∗ False.
+  Proof.
+    iIntros "(Hms & Hd & %Hcoh) Hreached Hpending".
+    rewrite /visit_reached_done /visit_pending.
+    iDestruct (own_valid_2 with "Hd Hreached") as %Hvd.
+    apply auth_both_valid_discrete in Hvd as [Hincl_d _].
+    apply singleton_included_l in Hincl_d as (xd & Hxd & _).
+    assert (d !! γ ≠ None) as Hdγ.
+    { intros Heq. rewrite Heq in Hxd. inversion Hxd. }
+    destruct (Hcoh γ Hdγ) as (n' & Hmγ).
+    iDestruct (own_valid_2 with "Hms Hpending") as %Hvm.
+    apply auth_both_valid_discrete in Hvm as [Hincl_m _].
+    apply singleton_included_l in Hincl_m as (ym & Hym & Hle).
+    iPureIntro. destruct Hmγ as [Hmγ | Hmγ]; rewrite Hmγ in Hym;
+      apply Some_equiv_inj in Hym; rewrite -Hym in Hle;
+      apply Some_included in Hle as [Heq | Hle].
+    - destruct Heq as [_ Hv]. apply (inj to_agree) in Hv. by inversion Hv.
+    - apply dfrac_agree_included in Hle as [_ Heqv]. by inversion Heqv.
+    - destruct Heq as [_ Hv]. apply (inj to_agree) in Hv. by inversion Hv.
+    - apply dfrac_agree_included in Hle as [_ Heqv]. by inversion Heqv.
+  Qed.
+
+  Lemma visited_agree_n γ n1 n2 :
+    (visit_done γ n1 ∨ visit_finished γ n1) -∗
+    (visit_done γ n2 ∨ visit_finished γ n2) -∗
+    ⌜n1 = n2⌝ ∗
+    (visit_done γ n1 ∨ visit_finished γ n1) ∗
+    (visit_done γ n2 ∨ visit_finished γ n2).
+  Proof.
+    iIntros "H1 H2".
+    iAssert (visit_reached_done γ n1) as "#R1".
+    { iDestruct "H1" as "[[_ $]|[_ $]]". }
+    iAssert (visit_reached_done γ n2) as "#R2".
+    { iDestruct "H2" as "[[_ $]|[_ $]]". }
+    iSplit. iApply (visited_reached_done_agree with "R1 R2").
+    iFrame.
+  Qed.
+
+End visited_map_res.
+
+Definition lg_mapUR := authR (gmapUR loc (agreeR (leibnizO gname))).
+Class lg_mapG Σ := Lg_mapG { lg_map_inG :> inG Σ lg_mapUR; lg_mapG_name : gname }.
+
+Section lg_map.
+  Context `{!lg_mapG Σ}.
+
+  Definition lg_mapg_type := gmap loc (agree gname).
+
+  Definition lg_mapg_auth (m : lg_mapg_type) : iProp Σ :=
+    own lg_mapG_name (● m).
+
+  Definition lg_mapg_frag l γ : iProp Σ :=
+    own lg_mapG_name (◯ {[ l := to_agree γ ]}).
+
+  Lemma lg_mapg_agree l γ1 γ2 :
+    lg_mapg_frag l γ1 -∗ lg_mapg_frag l γ2 -∗ ⌜γ1 = γ2⌝ ∗ lg_mapg_frag l γ1 ∗ lg_mapg_frag l γ2.
+  Proof.
+    rewrite /lg_mapg_frag. iIntros "H1 H2".
+    iDestruct (own_valid_2 with "H1 H2") as %Hv.
+    iFrame. iPureIntro.
+    rewrite -auth_frag_op auth_frag_valid singleton_op singleton_valid in Hv.
+    fold_leibniz. by apply to_agree_op_inv_L in Hv.
+  Qed.
+
+  Lemma lg_mapg_insert m l γ :
+    m !! l = None →
+    lg_mapg_auth m ==∗ lg_mapg_auth (<[ l:= to_agree γ ]> m) ∗ lg_mapg_frag l γ.
+  Proof.
+    rewrite /lg_mapg_auth /lg_mapg_frag. iIntros (Hfresh) "H".
+    iMod (own_update with "H") as "[$ $]"; last done.
+    apply auth_update_alloc.
+    by apply alloc_singleton_local_update.
+  Qed.
+
+End lg_map.
+
+Definition mapUR := authR (gmapUR val (dfrac_agreeR valO)).
+Class mapG Σ := MapG { map_inG :> inG Σ mapUR; mapG_name : gname }.
+
+Section map_res.
+  Context `{!mapG Σ}.
+
+  Definition mapg_type := gmap val (dfrac_agreeR valO).
+
+  Definition mapg_auth (m : mapg_type) : iProp Σ :=
+    own mapG_name (● m).
+
+  Definition mapg_insert_def (m : mapg_type) k v : mapg_type :=
+    <[ k := to_frac_agree 1 v ]> m.
+
+  (* A fragment with fraction [q] for key [k] and value [v]. A full fraction
+     [q = 1] gives exclusive ownership and permits removal. The caller may
+     split a full fragment into [n] pieces of fraction [1/n] via [mapg_split]. *)
+  Definition mapg_frag (k : val) (q : Qp) (v : val) : iProp Σ :=
+    own mapG_name (◯ {[ k := to_frac_agree q v ]}).
+
+  Lemma mapg_frag_op k q1 q2 v :
+    mapg_frag k (q1 + q2) v ⊣⊢ mapg_frag k q1 v ∗ mapg_frag k q2 v.
+  Proof.
+    rewrite /mapg_frag -own_op -auth_frag_op singleton_op.
+    by rewrite -frac_agree_op.
+  Qed.
+
+  Lemma mapg_frag_split k q1 q2 v :
+    mapg_frag k (q1 + q2) v -∗ mapg_frag k q1 v ∗ mapg_frag k q2 v.
+  Proof. iIntros "H". by iApply mapg_frag_op. Qed.
+
+  Lemma mapg_frag_combine k q1 q2 v :
+    mapg_frag k q1 v -∗ mapg_frag k q2 v -∗ mapg_frag k (q1 + q2) v.
+  Proof. iIntros "H1 H2". rewrite mapg_frag_op. iFrame. Qed.
+
+  Lemma mapg_frag_agree k q1 q2 v1 v2 :
+    mapg_frag k q1 v1 -∗ mapg_frag k q2 v2 -∗ ⌜v1 = v2⌝.
+  Proof.
+    rewrite /mapg_frag. iIntros "H1 H2".
+    iDestruct (own_valid_2 with "H1 H2") as %Hv.
+    iPureIntro.
+    rewrite -auth_frag_op auth_frag_valid singleton_op singleton_valid in Hv.
+    apply dfrac_agree_op_valid_L in Hv as [_ ?]. done.
+  Qed.
+
+  Lemma mapg_insert m k v :
+    m !! k = None →
+    mapg_auth m ==∗ mapg_auth (mapg_insert_def m k v) ∗ mapg_frag k 1 v.
+  Proof.
+    rewrite /mapg_auth /mapg_frag. iIntros (Hfresh) "H".
+    iMod (own_update with "H") as "[$ $]"; last done.
+    apply auth_update_alloc.
+    apply alloc_singleton_local_update; done.
+  Qed.
+
+  Lemma mapg_subset m k q v :
+    mapg_auth m -∗ mapg_frag k q v -∗
+      ⌜∃ y, m !! k ≡ Some y ∧ y.2 ≡ to_agree v⌝.
+  Proof.
+    rewrite /mapg_auth /mapg_frag. iIntros "H1 H2".
+    iDestruct (own_valid_2 with "H1 H2") as %Hv. iPureIntro.
+    apply auth_both_valid_discrete in Hv as [Hincl Hv].
+    apply singleton_included_l in Hincl as (y & Hy & Hle).
+    assert (✓ y) as Hvy.
+    { eapply (lookup_valid_Some _ k); [done|by rewrite Hy]. }
+    destruct y as [d a]. simpl.
+    apply Some_included in Hle as [Heq | Hinc].
+    - destruct Heq as [_ Heq2]. simpl in Heq2.
+      exists (d, a). split; [done|]. by symmetry.
+    - apply pair_included in Hinc as [_ Ha].
+      destruct Hvy as [_ Hva].
+      apply (agree_valid_included _ _ Hva) in Ha.
+      exists (d, a). split; [done|by symmetry].
+  Qed.
+
+  Lemma mapg_remove m k v :
+    mapg_auth m -∗ mapg_frag k 1 v ==∗ mapg_auth (delete k m).
+  Proof.
+    rewrite /mapg_auth /mapg_frag. iIntros "H1 H2".
+    iCombine "H1 H2" as "H".
+    iMod (own_update with "H") as "$"; last done.
+    apply auth_update_dealloc.
+    by apply delete_singleton_local_update, _.
+  Qed.
+
+End map_res.
+
+Definition capUR := authR (gmapUR nat (agreeR natO)).
+Class capG Σ := CapG { cap_inG :> inG Σ capUR; capG_name : gname }.
+
+Section cap_res.
+  Context `{!capG Σ}.
+
+  Definition cap_type := gmap nat (agree nat).
+
+  Definition cap_auth (m : cap_type) : iProp Σ :=
+    own capG_name (● m).
+
+  Definition cap_frag (id n : nat) : iProp Σ :=
+    own capG_name (◯ {[ id := to_agree n ]}).
+
+  Global Instance cap_frag_persistent id n : Persistent (cap_frag id n).
+  Proof. apply _. Qed.
+
+  Lemma cap_frag_agree id n1 n2 :
+    cap_frag id n1 -∗ cap_frag id n2 -∗ ⌜n1 = n2⌝.
+  Proof.
+    rewrite /cap_frag. iIntros "H1 H2".
+    iDestruct (own_valid_2 with "H1 H2") as %Hv. iPureIntro.
+    rewrite -auth_frag_op auth_frag_valid singleton_op singleton_valid in Hv.
+    fold_leibniz. by apply to_agree_op_inv_L in Hv.
+  Qed.
+
+  Lemma cap_insert m id n :
+    m !! id = None →
+    cap_auth m ==∗ cap_auth (<[ id := to_agree n ]> m) ∗ cap_frag id n.
+  Proof.
+    rewrite /cap_auth /cap_frag. iIntros (Hfresh) "H".
+    iMod (own_update with "H") as "[$ $]"; last done.
+    apply auth_update_alloc.
+    by apply alloc_singleton_local_update.
+  Qed.
+
+End cap_res.
+
+Definition idcntrUR := authUR nat.
+Class idcntrG Σ := IdcntrG { idcntr_inG :> inG Σ idcntrUR; idcntrG_name : gname }.
+
+Section idcntr.
+  Context `{!idcntrG Σ}.
+
+  Definition id_frag (id : nat) := own idcntrG_name (●{DfracOwn (1/2)} id).
+
+  Lemma id_agree id id' :
+    id_frag id -∗ id_frag id' -∗ ⌜id = id'⌝ ∗ id_frag id ∗ id_frag id'.
+  Proof.
+    rewrite /id_frag. iIntros "H1 H2". iCombine "H1 H2" as "H".
+    iDestruct (own_valid with "H") as %Hv.
+    apply auth_auth_dfrac_op_valid in Hv as [_ [Heq _]].
+    iDestruct "H" as "[H1 H2]". iFrame.
+    iPureIntro. apply leibniz_equiv. exact Heq.
+  Qed.
+
+  Lemma id_update id id' (Hle : id ≤ id') :
+    id_frag id -∗ id_frag id ==∗ id_frag id' ∗ id_frag id'.
+  Proof.
+    rewrite /id_frag. iIntros "H1 H2". iCombine "H1 H2" as "H".
+    iMod (own_update with "H") as "H".
+    { apply (auth_update_auth id id' (id' - id)).
+      apply (nat_local_update id 0 id' (id' - id)). lia. }
+    iDestruct "H" as "[H1 H2]". iFrame. done.
+  Qed.
+
+End idcntr.
